WIP

code/ecdsa/Hacl.Impl.EC.Masking.fst
@@ -165,6 +165,15 @@ let isZero_uint64_CT #c f =
   pop_frame();
   r
 
+inline_for_extraction noextract
+val isZero_uint64_nCT: #c: curve -> f: felem c -> Stack bool
+  (requires fun h -> live h f)
+  (ensures fun h0 r h1 -> modifies0 h0 h1 /\ r = (as_nat c h0 f = 0))
+
+let isZero_uint64_nCT f =
+  let f = isZero_uint64_CT f in 
+  Hacl.Impl.P256.LowLevel.RawCmp.eq_u64_nCT f (u64 0xffffffffffffffff)
+
 
 val compare_felem: #c: curve -> a: felem c -> b: felem c -> Stack uint64
   (requires fun h -> live h a /\ live h b)
